test/generated2.dfy
@@ -1,18 +1,47 @@
-
-
 datatype tree<a1> =  Node(a1, tree<a1>, tree<a1>) |  Nil
-function repr(xre : tree<int>) : tree<int> decreases xre {xre}
-function spec(xsp : tree<int>) : int decreases xsp {f(0, xsp)}
-function f(x5 : int, x6 : tree<int>) : int decreases x6
-  {match x6
-case Nil =>  x5
-case Node(a, l, r) =>  ((sum) => f(sum + a, r))(
-                                                  f(x5, l))}
-function target(xtarg : tree<int>) : int decreases xtarg
-  {match xtarg
-case Nil =>  0
-case Node(a, l, r) =>  join(a, target(l),
-                                                    target(r))}
-function s0() : int  {0}
-function join(x2 : int, x3 : int, x4 : int) : int decreases x4 {x3 + x2 + x4}
-lemma correctness_lemma(x : tree<int>)  ensures (target(x) == spec(repr(x))) {}
+
+function repr(xre : tree<int>) : tree<int>
+decreases xre
+{
+  xre
+}
+
+function spec(xsp : tree<int>) : int
+decreases xsp
+{
+  f(0, xsp)
+}
+
+function f(x5 : int, x6 : tree<int>) : int
+decreases x6
+{
+  match x6
+  case Nil => x5
+  case Node(a, l, r) => ((sum) => f(sum + a, r))(f(x5, l))
+}
+
+function target(xtarg : tree<int>) : int
+decreases xtarg
+{
+  match xtarg
+  case Nil => 0
+  case Node(a, l, r) => join(a, target(l), target(r))
+}
+
+function s0() : int
+
+{
+  0
+}
+
+function join(x2 : int, x3 : int, x4 : int) : int
+decreases x4
+{
+  x3 + x2 + x4
+}
+
+lemma correctness_lemma(x : tree) 
+ensures (target(x) == spec(repr(x)))
+{
+  
+}
